src/Init/Data/Slice/Array/Iterator.lean
@@ -60,7 +60,6 @@ instance SubarrayIterator.instFinite : Finite (SubarrayIterator α) Id :=
   .of_finitenessRelation instFinitelessRelation
 
 instance [Monad m] : IteratorCollect (SubarrayIterator α) Id m := .defaultImplementation
-instance [Monad m] : IteratorCollectPartial (SubarrayIterator α) Id m := .defaultImplementation
 instance [Monad m] : IteratorLoop (SubarrayIterator α) Id m := .defaultImplementation
 instance [Monad m] : IteratorLoopPartial (SubarrayIterator α) Id m := .defaultImplementation
 
